add inference algo draft

SystemFD/Algorithm.lean
@@ -10,69 +10,240 @@ def wf_kind : Term -> Option Unit
   .some ()
 | _ => .none
 
-inductive InferKindVariant where
-| prf | wf
-
 @[simp]
-abbrev InferKindArgs : (v : InferKindVariant) -> Type
-| .prf => Ctx Term × Term
-| .wf => Ctx Term
-
-namespace InferKindArgs
-  @[simp]
-  def size1 : (v : InferKindVariant) -> InferKindArgs v -> Nat
-  | .prf, (_, t) => Term.size t
-  | .wf, _ => 0
-
-  @[simp]
-  def size2 : (v : InferKindVariant) -> InferKindArgs v -> Nat
-  | .prf, (Γ, _) => Γ.length + 1
-  | .wf, Γ => Γ.length
-
-end InferKindArgs
-
-@[simp]
-abbrev InferKindRet : (v : InferKindVariant) -> Type
-| .prf => Option Term
-| .wf => Option Unit
+def is_openm : Frame Term -> Option Term
+| .openm T => .some T
+| _ => .none
 
 @[simp]
 def is_const : Term -> Option Const
-| _ => sorry
+| .const K => .some K
+| _ => .none
+
+@[simp]
+def is_pointed : Term -> Option Unit
+| .const .pointed => .some ()
+| _ => .none
+
+@[simp]
+def is_unpointed : Term -> Option Unit
+| .const .unpointed => .some ()
+| _ => .none
 
 @[simp]
 def is_arrowk : Term -> Option (Term × Term)
-| _ => sorry
+| .arrowk A B => .some (A, B)
+| _ => .none
 
 @[simp]
-def infer_kind : (v : InferKindVariant) -> InferKindArgs v -> InferKindRet v
-| .prf, (Γ, #x) => do
-  let _ <- infer_kind .wf Γ
-  Frame.get_type (Γ d@ x)
-| .prf, (Γ, ∀[A] B) => do
+def is_arrow : Term -> Option (Term × Term)
+| .arrow A B => .some (A, B)
+| _ => .none
+
+@[simp]
+def is_eq : Term -> Option (Term × Term)
+| .eq A B => .some (A, B)
+| _ => .none
+
+@[simp]
+def is_appk : Term -> Option (Term × Term)
+| .appk A B => .some (A, B)
+| _ => .none
+
+
+@[simp]
+def is_all : Term -> Option (Term × Term)
+| .all A B => .some (A, B)
+| _ => .none
+
+@[simp]
+def infer_kind : Ctx Term -> Term -> Option Term
+| Γ, #x => do
+  let T <- Frame.get_type (Γ d@ x)
+  let _ <- wf_kind T
+  .some T
+| Γ, ∀[A] B => do
   let _ <- wf_kind A
-  let Bk <- infer_kind .prf (.kind A::Γ, B)
+  let Bk <- infer_kind (.kind A::Γ) B
   let _ <- wf_kind Bk
   .some Bk
-| .prf, (Γ, A -t> B) => do
-  let Ak <- infer_kind .prf (Γ, A)
+| Γ, A -t> B => do
+  let Ak <- infer_kind Γ A
   let _ <- is_const Ak
-  let Bk <- infer_kind .prf (Γ, B)
+  let Bk <- infer_kind Γ B
   let K <- is_const Bk
   .some (.const K)
-| .prf, (Γ, f `@k a) => do
-  let fk <- infer_kind .prf (Γ, f)
+| Γ, f `@k a => do
+  let fk <- infer_kind Γ f
   let (A, B) <- is_arrowk fk
-  let ak <- infer_kind .prf (Γ, a)
+  let ak <- infer_kind Γ a
   if A == ak then .some B else .none
-| .prf, (Γ, A ~ B) => do
-  let Ak <- infer_kind .prf (Γ, A)
-  let Bk <- infer_kind .prf (Γ, B)
+| Γ, A ~ B => do
+  let Ak <- infer_kind Γ A
+  let Bk <- infer_kind Γ B
   if Ak == ★ && Bk == ★ then .some ◯ else .none
+| _, _ => .none
+
+inductive InferTypeVariant where
+| prf | ctor
+
+@[simp]
+abbrev InferTypeArgs : (v : InferTypeVariant) -> Type
+| .prf => Ctx Term × Term
+| .ctor => Ctx Term × Term × Nat
+
+namespace InferTypeArgs
+  @[simp]
+  def size1 : (v : InferTypeVariant) -> InferTypeArgs v -> Nat
+  | .prf, (_, t) => Term.size t
+  | .ctor, (_, t, n) => Term.size t
+
+  @[simp]
+  def size2 : (v : InferTypeVariant) -> InferTypeArgs v -> Nat
+  | .prf, (_, t) => Term.size t
+  | .ctor, (_, t, n) => Term.size t + n + 1
+end InferTypeArgs
+
+@[simp]
+def infer_type : (v : InferTypeVariant) -> InferTypeArgs v -> Option Term
+| .prf, (Γ, .letdata T n t) => do
+  let _ <- wf_kind T
+  let A <- infer_type .ctor (.datatype T n::Γ, t, n)
+  .some A
+| .ctor, (Γ, .letctor T t, n + 1) => do
+  let Tk <- infer_kind Γ T
+  let _ <- is_pointed Tk
+  let A <- infer_type .ctor (.ctor T::Γ, t, n)
+  .some A
+| .ctor, (Γ, t, 0) => infer_type .prf (Γ, t)
+| .prf, (Γ, .letopentype T t) => do
+  let _ <- wf_kind T
+  let A <- infer_type .prf (.opent T::Γ, t)
+  .some A
+| .prf, (Γ, .letopen T t) => do
+  let Tk <- infer_kind Γ T
+  let _ <- is_const Tk
+  let A <- infer_type .prf (.openm T::Γ, t)
+  .some A
+| .prf, (Γ, .insttype T t) => do
+  let Tk <- infer_kind Γ T
+  let _ <- is_const Tk
+  let A <- infer_type .prf (.insttype T::Γ, t)
+  .some A
+| .prf, (Γ, .inst x t1 t2) => do
+  let T <- is_openm (Γ d@ x)
+  let T' <- infer_type .prf (Γ, t1)
+  let A <- infer_type .prf (.inst x t1::Γ, t2)
+  if T == T' then .some A else .none
+| .prf, (Γ, #x) => do
+  let T <- Frame.get_type (Γ d@ x)
+  let _ <- infer_kind Γ T
+  .some T
+| .prf, (Γ, .ite p s i e) => do
+  let A <- infer_type .prf (Γ, p)
+  let (τ, R) := Term.to_telescope A
+  let ctorid <- Term.neutral_head p
+  let dataid <- Term.neutral_head R
+  let Rk <- infer_kind Γ R
+  let _ <- is_pointed Rk
+  let R' <- infer_type .prf (Γ, s)
+  let B <- infer_type .prf (Γ, i)
+  let (τ', T) := Term.to_telescope B
+  let Tk <- infer_kind Γ T
+  let _ <- is_const Tk
+  let T' <- infer_type .prf (Γ, e)
+  if R == R'
+    && τ == τ'
+    && T == T'
+    && is_datatype Γ ctorid dataid
+  then .some T
+  else .none
+| .prf, (Γ, .guard p s t) => do
+  let A <- infer_type .prf (Γ, p)
+  let (τ, R) := Term.to_telescope A
+  let Rk <- infer_kind Γ R
+  let _ <- is_unpointed Rk
+  let R' <- infer_type .prf (Γ, s)
+  let B <- infer_type .prf (Γ, t)
+  let (τ', T) := Term.to_telescope B
+  let Tk <- infer_kind Γ T
+  let _ <- is_const Tk
+  if R == R' && τ == τ' then .some T else .none
+| .prf, (Γ, `λ[A] t) => do
+  let Ak <- infer_kind Γ A
+  let _ <- is_const Ak
+  let B <- infer_type .prf (.type A::Γ, t)
+  .some (A -t> B)
+| .prf, (Γ, f `@ a) => do
+  let T <- infer_type .prf (Γ, f)
+  let (A, B) <- is_arrow T
+  let A' <- infer_type .prf (Γ, a)
+  if A == A' then .some B else .none
+| .prf, (Γ, Λ[A] t) => do
+  let Ak <- infer_kind Γ A
+  let _ <- wf_kind Ak
+  let B <- infer_type .prf (.kind A::Γ, t)
+  .some (∀[A] B)
+| .prf, (Γ, f `@t a) => do
+  let T <- infer_type .prf (Γ, f)
+  let (A, B) <- is_all T
+  let A' <- infer_type .prf (Γ, a)
+  if A == A' then .some B else .none
+| .prf, (Γ, t ▹ c) => do
+  let A <- infer_type .prf (Γ, t)
+  let T <- infer_type .prf (Γ, c)
+  let (A', B) <- is_eq T
+  if A == A' then .some B else .none
+| .prf, (Γ, .refl A) => do
+  let Ak <- infer_kind Γ A
+  let _ <- wf_kind Ak
+  .some A
+| .prf, (Γ, .sym t) => do
+  let T <- infer_type .prf (Γ, t)
+  let (A, B) <- is_eq T
+  .some (B ~ A)
+| .prf, (Γ, t1 `; t2) => do
+  let T1 <- infer_type .prf (Γ, t1)
+  let T2 <- infer_type .prf (Γ, t2)
+  let (A, B) <- is_eq T1
+  let (B', C) <- is_eq T2
+  if B == B' then .some (A ~ C) else .none
+| .prf, (Γ, f `@c a) => do
+  let T1 <- infer_type .prf (Γ, f)
+  let T2 <- infer_type .prf (Γ, a)
+  let (A, B) <- is_eq T1
+  let (C, D) <- is_eq T2
+  .some ((A `@k C) ~ (B `@k D))
+| .prf, (Γ, t1 -c> t2) => do
+  let T1 <- infer_type .prf (Γ, t1)
+  let T2 <- infer_type .prf (Γ, t2)
+  let (A, B) <- is_eq T1
+  let (C, D) <- is_eq T2
+  .some ((A -t> C) ~ (B -t> D))
+| .prf, (Γ, .fst t) => do
+  let T <- infer_type .prf (Γ, t)
+  let (U, V) <- is_eq T
+  let (A, C) <- is_appk U
+  let (B, D) <- is_appk V
+  .some (A ~ B)
+| .prf, (Γ, .snd t) => do
+  let T <- infer_type .prf (Γ, t)
+  let (U, V) <- is_eq T
+  let (A, C) <- is_appk U
+  let (B, D) <- is_appk V
+  .some (C ~ D)
+| .prf, (Γ, ∀c[K] t) => do
+  let T <- infer_type .prf (Γ, t)
+  let (A, B) <- is_eq T
+  .some ((∀[K] A) ~ (∀[K] B))
+| .prf, (Γ, f `@c[a]) => do
+  let T1 <- infer_type .prf (Γ, f)
+  let T2 <- infer_type .prf (Γ, a)
+  let (U, V) <- is_eq T1
+  let (K1, A) <- is_all U
+  let (K2, B) <- is_all V
+  let (C, D) <- is_eq T2
+  if K1 == K2 then .some ((A β[C]) ~ (B β[D])) else .none
 | .prf, _ => .none
-| .wf, [] => .some ()
-| .wf, (.cons (.kind A) Γ) => do
-  let _ <- wf_kind A
-  infer_kind .wf Γ
-| .wf, (.cons _ Γ) => infer_kind .wf Γ
-termination_by v args => (InferKindArgs.size1 v args, InferKindArgs.size2 v args)
+| .ctor, _ => .none
+termination_by v t => (InferTypeArgs.size1 v t, InferTypeArgs.size2 v t)
