SystemFD/Algorithm/Soundness.lean
@@ -1,0 +1,88 @@
+import SystemFD.Term
+import SystemFD.Judgment
+import SystemFD.Ctx
+import SystemFD.Algorithm
+
+theorem wf_kind_sound : wf_kind t = .some u -> ⊢ Γ -> Γ ⊢ t : .kind := by
+intro h wf
+induction t using wf_kind.induct
+case _ K => constructor; apply wf
+case _ A B ih1 ih2 =>
+  simp at h; rw [Option.bind_eq_some] at h
+  cases h; case _ u1 h =>
+  simp at h; rw [Option.bind_eq_some] at h
+  cases h; case _ h1 h2 =>
+  cases h2; case _ u2 h2 =>
+  constructor; apply ih1 h1; apply ih2 h2.1
+case _ t h1 h2 =>
+  exfalso
+  cases t <;> simp at h
+  case _ => apply h1 _ rfl
+  case _ => apply h2 _ _ rfl
+
+-- @[simp]
+-- abbrev InferKindSoundType : (v:InferKindVariant) -> InferKindArgs v -> InferKindRet v -> Prop
+-- | .prf, (Γ, t), A =>  Γ ⊢ t : A
+-- | .wf, Γ, () => ⊢ Γ
+
+theorem infer_kind_sound : infer_kind Γ t = .some A -> ⊢ Γ -> Γ ⊢ t : A := by
+intro h wf
+induction Γ, t using infer_kind.induct generalizing A
+case _ Γ x =>
+  simp at h; rw [Option.bind_eq_some] at h
+  cases h; case _ u1 h =>
+  cases h; case _ h1 h2 =>
+  simp at h2; rw [Option.bind_eq_some] at h2
+  cases h2; case _ u2 h2 =>
+    constructor; apply wf
+    rw [h2.2] at h1; rw [h1]
+case _ Γ A' B ih =>
+  simp at h; rw [Option.bind_eq_some] at h
+  cases h; case _ u1 h =>
+  cases h; case _ h1 h2 =>
+  simp at h2; rw [Option.bind_eq_some] at h2
+  cases h2; case _ u2 h2 =>
+  cases h2; case _ h2 h3 =>
+  simp at h3; rw [Option.bind_eq_some] at h3
+  cases h3; case _ u3 h3 =>
+  cases h3; case _ h3 h4 =>
+    injection h4 with e; subst e
+    have lem1 := wf_kind_sound h1 wf
+    have lem2 : ⊢ (.kind A' :: Γ) := by
+      constructor; apply lem1; apply wf
+    constructor; apply lem1
+    apply ih h2; apply lem2
+    apply wf_kind_sound h3 wf
+case _ Γ A' B ih1 ih2 =>
+  simp at h; rw [Option.bind_eq_some] at h
+  cases h; case _ u1 h =>
+  cases h; case _ h1 h2 =>
+  rw [Option.bind_eq_some] at h2
+  cases h2; case _ u2 h2 =>
+  cases h2; case _ h2 h3 =>
+  rw [Option.bind_eq_some] at h3
+  cases h3; case _ u3 h3 =>
+  cases h3; case _ h3 h4 =>
+  rw [Option.bind_eq_some] at h4
+  cases h4; case _ u4 h4 =>
+  cases h4; case _ h4 h5 =>
+  cases u1 <;> simp at h2; case _ u1 =>
+  cases u3 <;> simp at h4; case _ u3 =>
+    injection h5 with e
+    subst e; subst h2; subst h4
+    constructor; apply ih1 h1 wf; apply ih2 h3 wf
+case _ Γ f a ih1 ih2 =>
+  simp at h; rw [Option.bind_eq_some] at h
+  cases h; case _ u1 h =>
+  cases h; case _ h1 h2 =>
+  rw [Option.bind_eq_some] at h2
+  cases h2; case _ u2 h2 =>
+  cases h2; case _ h2 h3 =>
+  rw [Option.bind_eq_some] at h3
+  cases h3; case _ u3 h3 =>
+  cases h3; case _ h3 h4 =>
+    sorry
+case _ => sorry
+case _ Γ t h1 h2 h3 h4 h5 =>
+  exfalso
+  cases t <;> simp at *
